Day 2 part 1, no verification, learned about for-loops, multisets, and vscode-dafny loves to reformat indention

problems/2/Problem2.dfy
@@ -1,6 +1,75 @@
+include "../../parser/split.dfy"
+include "../../parser/parseInt.dfy"
+include "../../libraries/src/dafny/Collections/Seqs.dfy"
+
 module Problem2 {
+
+    import opened Split
+    import opened ParseInt
+    import opened Dafny.Collections.Seq
+    
+    datatype Cube = Red | Green | Blue
+    datatype Game = Game(id: int, cubes: seq<multiset<Cube>> )
+
+    predicate possibleGame(a: seq<multiset<Cube>>, b: multiset<Cube>) 
+    {
+        forall i :: 0 <= i < |a| ==> a[i] <= b
+    }
+
+    // This can be a Fold * Map ? Composable?
+    method findAmount(g: seq<seq<string>>) returns (gameList: seq<multiset<Cube>>)
+    { 
+        // TODO - Implement in a Fold
+        for i := 0 to |g| 
+        {
+            var s := Map(c => split(c, " "), g[i]);
+            // TODO - Implement in a Map
+            var colorSet: multiset<Cube> := multiset{};
+            for j := 0 to |s|
+            {
+                var numberOfColors := Integer(s[j][1]);
+                var color: Cube := match s[j][2] 
+                {
+                    case "red" => Red
+                    case "green" => Green
+                    case "blue" => Blue
+                    case _ => Red
+                };
+                colorSet := colorSet[color :=  numberOfColors];
+            }
+            gameList := gameList + [colorSet];
+        }
+        return gameList;
+    }
+
     method problem2_1(input: string) returns (x: int) {
-        return 3;
+        var lines := Filter(line => line != "", splitOnBreak(input));
+
+        //Split by game
+        var games := Map(game => split(game, ":"), lines);
+                  // Parse game lists
+                  var listGames: seq<Game> := [];
+                for i := 0 to |games| 
+        {
+            var  grabbed := Map(hands => split(hands,";"), games[i][1..]);
+            var game := Map(g => split(g, ","),grabbed[0]);
+            var bag := findAmount(game);
+            listGames := listGames + [Game(id := i + 1, cubes := bag)];
+        }
+        
+        //Find the games that adhere to limit
+        var limit: multiset<Cube> := multiset{};
+        limit := limit[Blue := 14];
+        limit := limit[Red := 12];
+        limit := limit[Green := 13];
+        var results := Filter((g: Game) => possibleGame(g.cubes, limit),listGames);
+        
+        //Get sum of Ids
+        for j := 0 to |results|
+        {
+            x := x + results[j].id; 
+        }
+        return x;
     }
 
     method problem2_2(input: string) returns (x: int) {
